pulse/share/steel/examples/pulse/dice/L0Impl.fst
@@ -1,0 +1,352 @@
+module L0Impl
+module R = Steel.ST.Reference
+module A = Steel.ST.Array
+module T = FStar.Tactics
+module PM = Pulse.Main
+open Steel.ST.Util 
+open Steel.ST.Array
+open Steel.FractionalPermission
+open FStar.Ghost
+open Pulse.Steel.Wrapper
+module A = Steel.ST.Array
+module US = FStar.SizeT
+module U8 = FStar.UInt8
+module U32 = FStar.UInt32
+open HACL
+open L0Types
+open L0Crypto
+
+```pulse
+fn get_witness (x:A.array U8.t) (#y:Ghost.erased (Seq.seq U8.t))
+requires A.pts_to x full_perm y
+returns z:Ghost.erased (Seq.seq U8.t)
+ensures A.pts_to x full_perm y ** pure (y==z)
+{   
+    y
+}
+```
+
+
+(* ------- L0 CORE STEP 1 ------- *)
+
+let l0_repr_post_state (vl0:l0_repr) (s1 s2 s3 s4 s5:_) 
+  = { vl0 with 
+      deviceID_pub = s1;
+      deviceID_priv = s2;
+      aliasKey_pub = s3;
+      aliasKey_priv = s4;
+      authKeyID = s5;
+    }
+
+let l0_core_step1_post
+  (l0: l0_record)
+  (vl0: l0_repr)
+  (alg:alg_t)
+  : prop = 
+    valid_hkdf_ikm_len (digest_len alg) /\
+    derive_DeviceID_spec alg (digest_len alg) vl0.cdi l0.deviceID_label_len vl0.deviceID_label
+      == (vl0.deviceID_pub, vl0.deviceID_priv) /\
+    derive_AliasKey_spec alg (digest_len alg) vl0.cdi vl0.fwid l0.aliasKey_label_len vl0.aliasKey_label
+      == (vl0.aliasKey_pub, vl0.aliasKey_priv) /\
+    derive_authKeyID_spec alg vl0.deviceID_pub
+      == vl0.authKeyID 
+
+```pulse
+fn l0_core_step1
+  (l0: l0_record)
+  (#vl0: Ghost.erased l0_repr)
+  requires (
+    l0_perm l0 vl0 `star`
+    pure(valid_hkdf_lbl_len l0.deviceID_label_len /\
+         valid_hkdf_lbl_len l0.aliasKey_label_len)
+  )
+  ensures (
+    exists (vl0_:l0_repr). 
+      l0_perm l0 vl0_ **
+      pure (l0_core_step1_post l0 vl0_ dice_hash_alg)
+  )
+{
+  dice_digest_len_is_hkdf_ikm;
+
+  rewrite (l0_perm l0 vl0)
+    as (
+      A.pts_to l0.cdi full_perm vl0.cdi `star`
+      A.pts_to l0.fwid full_perm vl0.fwid `star`
+      A.pts_to l0.deviceID_label full_perm vl0.deviceID_label `star`
+      A.pts_to l0.aliasKey_label full_perm vl0.aliasKey_label `star`
+      A.pts_to l0.deviceID_pub full_perm vl0.deviceID_pub `star`
+      A.pts_to l0.deviceID_priv full_perm vl0.deviceID_priv `star`
+      A.pts_to l0.aliasKey_pub full_perm vl0.aliasKey_pub `star`
+      A.pts_to l0.aliasKey_priv full_perm vl0.aliasKey_priv `star`
+      A.pts_to l0.deviceIDCSR_buf full_perm vl0.deviceIDCSR_buf `star`
+      A.pts_to l0.aliasKeyCRT_buf full_perm vl0.aliasKeyCRT_buf `star`
+      A.pts_to l0.authKeyID full_perm vl0.authKeyID
+    );
+
+  derive_DeviceID dice_hash_alg l0.deviceID_pub l0.deviceID_priv l0.cdi l0.deviceID_label_len l0.deviceID_label;
+  derive_AliasKey dice_hash_alg l0.aliasKey_pub l0.aliasKey_priv l0.cdi l0.fwid l0.aliasKey_label_len l0.aliasKey_label;
+  derive_authkeyID dice_hash_alg l0.authKeyID l0.deviceID_pub;
+
+  let s1 = get_witness (l0.deviceID_pub);
+  let s2 = get_witness (l0.deviceID_priv);
+  let s3 = get_witness (l0.aliasKey_pub);
+  let s4 = get_witness (l0.aliasKey_priv);
+  let s5 = get_witness (l0.authKeyID);
+
+  rewrite (
+    A.pts_to l0.cdi full_perm vl0.cdi `star`
+    A.pts_to l0.fwid full_perm vl0.fwid `star`
+    A.pts_to l0.deviceID_label full_perm vl0.deviceID_label `star`
+    A.pts_to l0.aliasKey_label full_perm vl0.aliasKey_label `star`
+    A.pts_to l0.deviceID_pub full_perm s1 `star`
+    A.pts_to l0.deviceID_priv full_perm s2 `star`
+    A.pts_to l0.aliasKey_pub full_perm s3 `star`
+    A.pts_to l0.aliasKey_priv full_perm s4 `star`
+    A.pts_to l0.deviceIDCSR_buf full_perm vl0.deviceIDCSR_buf `star`
+    A.pts_to l0.aliasKeyCRT_buf full_perm vl0.aliasKeyCRT_buf `star`
+    A.pts_to l0.authKeyID full_perm s5
+  ) as (l0_perm l0 (l0_repr_post_state vl0 s1 s2 s3 s4 s5));
+  ()
+}
+```
+
+(* ------- L0 CORE STEP 2 ------- *)
+
+assume
+val length_of_deviceIDCSR (len: U32.t) : U32.t 
+
+assume
+val len_of_deviceIDCRI
+  (version: U32.t)
+  (s_common: string)
+  (s_org: string)
+  (s_country: string)
+  : U32.t
+
+assume
+val serialize_deviceIDCSR 
+  (deviceIDCRI_len: U32.t)
+  (deviceIDCSR: deviceIDCSR_t deviceIDCRI_len)
+  : Seq.seq U8.t
+
+assume
+val serialize_deviceIDCRI 
+  (deviceIDCRI: deviceIDCRI_t)
+  : Seq.seq U8.t
+
+assume 
+val sign_and_finalize_deviceIDCSR_spec
+  (deviceID_priv: Seq.seq U8.t)
+  (deviceIDCRI_len: U32.t)
+  (deviceIDCRI_seq: Seq.seq U8.t)
+  : deviceIDCSR_t deviceIDCRI_len
+
+assume
+val create_deviceIDCRI_spec
+  (version: U32.t)
+  (s_common: string)
+  (s_org: string)
+  (s_country: string)
+  (ku: U32.t)
+  (deviceID_pub: Seq.seq U8.t)
+  : deviceIDCRI_t
+
+```pulse
+fn create_deviceIDCRI
+  (l0: l0_record)
+  (deviceIDCSR: deviceIDCSR_ingredients_t)
+  (aliasKeyCRT: aliasKeyCRT_ingredients_t)
+  (#vl0: Ghost.erased l0_repr)
+  requires pure (l0.deviceIDCRI_len = len_of_deviceIDCRI 
+                                        deviceIDCSR.version 
+                                        deviceIDCSR.s_common 
+                                        deviceIDCSR.s_org 
+                                        deviceIDCSR.s_country)
+  ensures pure (Seq.equal 
+    (serialize_deviceIDCRI (create_deviceIDCRI_spec
+                              deviceIDCSR.version
+                              deviceIDCSR.s_common
+                              deviceIDCSR.s_org
+                              deviceIDCSR.s_country
+                              deviceIDCSR.ku
+                              vl0.deviceID_pub))
+    vl0.deviceIDCRI_buf
+  )
+{
+  admit()
+(* 
+
+(* Create deviceIDCRI *)
+  let deviceID_pub32: B32.lbytes32 32ul = B32.of_buffer 32ul deviceID_pub in
+
+  printf "Creating AliasKey Certificate TBS Message\n" done;
+  let deviceIDCRI: deviceIDCRI_t = x509_get_deviceIDCRI
+                                                                    csr_version
+                                                                    s_common
+                                                                    s_org
+                                                                    s_country
+                                                                    ku
+                                                                    deviceID_pub32 in
+
+  (* Prf *) lemma_serialize_deviceIDCRI_size_exact deviceIDCRI;
+
+  printf "Serializing AliasKey Certificate TBS\n" done;
+(* Serialize deviceIDCRI *)
+  let offset = serialize32_deviceIDCRI_backwards
+                 deviceIDCRI
+                 deviceIDCRI_buf
+                 deviceIDCRI_len in
+
+  HST.pop_frame ()
+
+*)
+}
+```
+
+
+
+let l0_core_step2_pre
+  (l0: l0_record)
+  (deviceIDCSR: deviceIDCSR_ingredients_t)
+  (aliasKeyCRT: aliasKeyCRT_ingredients_t)
+  : prop = 
+  // let deviceIDCRI_len = len_of_deviceIDCRI
+  //                         deviceIDCSR.version
+  //                         deviceIDCSR.s_common
+  //                         deviceIDCSR.s_org
+  //                         deviceIDCSR.s_country in
+  U32.(0ul <^ l0.deviceIDCRI_len) /\ 
+  valid_deviceIDCSR_ingredients l0.deviceIDCRI_len /\
+  l0.deviceIDCSR_len == length_of_deviceIDCSR l0.deviceIDCRI_len
+
+
+let l0_core_step2_post
+  (l0: l0_record)
+  (deviceIDCSR: deviceIDCSR_ingredients_t)
+  (aliasKeyCRT: aliasKeyCRT_ingredients_t)
+  (vl0: Ghost.erased l0_repr)
+  : prop = 
+  // let deviceIDCRI_len = len_of_deviceIDCRI
+  //                         deviceIDCSR.version
+  //                         deviceIDCSR.s_common
+  //                         deviceIDCSR.s_org
+  //                         deviceIDCSR.s_country in
+  let deviceIDCRI = create_deviceIDCRI_spec
+                      deviceIDCSR.version
+                      deviceIDCSR.s_common
+                      deviceIDCSR.s_org
+                      deviceIDCSR.s_country
+                      deviceIDCSR.ku
+                      vl0.deviceID_pub in
+  let deviceIDCRI_seq = serialize_deviceIDCRI deviceIDCRI in
+  let deviceIDCSR = sign_and_finalize_deviceIDCSR_spec
+                      vl0.deviceID_priv
+                      l0.deviceIDCRI_len
+                      deviceIDCRI_seq in
+  vl0.deviceIDCSR_buf == serialize_deviceIDCSR l0.deviceIDCRI_len deviceIDCSR
+
+```pulse
+fn l0_core_step2
+  (l0: l0_record)
+  (deviceIDCSR: deviceIDCSR_ingredients_t)
+  (aliasKeyCRT: aliasKeyCRT_ingredients_t)
+  (#vl0: Ghost.erased l0_repr)
+  requires (
+    l0_perm l0 vl0 **
+    pure (l0_core_step2_pre l0 deviceIDCSR aliasKeyCRT)
+  )
+  ensures (
+    exists (vl0_:l0_repr). 
+      l0_perm l0 vl0_ **
+      pure (l0_core_step2_post l0 deviceIDCSR aliasKeyCRT vl0_)
+  )
+{
+  let deviceIDCRI_len = len_of_deviceIDCRI
+                        deviceIDCSR.version
+                        deviceIDCSR.s_common
+                        deviceIDCSR.s_org
+                        deviceIDCSR.s_country;
+  // TOOD: assign l0.deviceIDCRI_len = deviceIDCRI_len
+  let deviceIDCRI_buf = new_array 0uy (u32_to_us l0.deviceIDCRI_len);
+  admit()
+(*
+  create_deviceIDCRI
+    (* version   *) csr_version
+                    s_common
+                    s_org
+                    s_country
+                    ku
+    (* DeviceID  *) deviceID_pub
+    (*DeviceIDCRI*) deviceIDCRI_len
+                    deviceIDCRI_buf;
+  (**) let hs2 = HST.get () in
+
+  (**) assert (
+    let deviceIDCRI: deviceIDCRI_t = create_deviceIDCRI_spec
+                                                                      (csr_version)
+                                                                      (s_common)
+                                                                      (s_org)
+                                                                      (s_country)
+                                                                      (ku)
+                                                                      (B.as_seq h0 deviceID_pub) in
+    (* Prf *) lemma_serialize_deviceIDCRI_size_exact deviceIDCRI;
+    B.as_seq hs2 deviceIDCRI_buf == serialize_deviceIDCRI `serialize` deviceIDCRI
+  );
+
+  (**) B.modifies_trans B.loc_none h0 hs1 (B.loc_buffer deviceIDCRI_buf) hs2;
+  (**) B.modifies_buffer_elim deviceID_priv (B.loc_buffer deviceIDCRI_buf) h0 hs2;
+  printf "Signing and finalizing DeviceID Certificate Signing Request\n" done;
+  sign_and_finalize_deviceIDCSR
+    (*Signing Key*) deviceID_priv
+    (*DeviceIDCRI*) deviceIDCRI_len
+                    deviceIDCRI_buf
+    (*DeviceIDCSR*) deviceIDCSR_len
+                    deviceIDCSR_buf;
+  (**) let hs3 = HST.get () in
+
+  (**) assert (
+    let deviceIDCSR: deviceIDCSR_t deviceIDCRI_len = sign_and_finalize_deviceIDCSR_spec
+                                                                      (B.as_seq h0 deviceID_priv)
+                                                                      (deviceIDCRI_len)
+                                                                      (B.as_seq hs2 deviceIDCRI_buf) in
+    (* Prf *) lemma_serialize_deviceIDCSR_size_exact deviceIDCRI_len deviceIDCSR;
+    B.as_seq hs3 deviceIDCSR_buf == serialize_deviceIDCSR deviceIDCRI_len `serialize` deviceIDCSR
+  );
+
+  (**) assert (
+    let deviceIDCRI_len: asn1_TLV_int32_of_type SEQUENCE = len_of_deviceIDCRI
+                                                            csr_version
+                                                            s_common
+                                                            s_org
+                                                            s_country in
+    let deviceIDCRI: deviceIDCRI_t = create_deviceIDCRI_spec
+                                                                      (csr_version)
+                                                                      (s_common)
+                                                                      (s_org)
+                                                                      (s_country)
+                                                                      (ku)
+                                                                      (B.as_seq h0 deviceID_pub) in
+    let deviceIDCRI_seq = serialize_deviceIDCRI `serialize` deviceIDCRI in
+    let (* Prf *) _ = lemma_serialize_deviceIDCRI_size_exact deviceIDCRI in
+    let deviceIDCSR: deviceIDCSR_t deviceIDCRI_len = sign_and_finalize_deviceIDCSR_spec
+                                                                      (B.as_seq h0 deviceID_priv)
+                                                                      (deviceIDCRI_len)
+                                                                      (deviceIDCRI_seq) in
+    (* Prf *) lemma_serialize_deviceIDCSR_size_exact deviceIDCRI_len deviceIDCSR;
+    B.as_seq hs3 deviceIDCSR_buf == serialize_deviceIDCSR deviceIDCRI_len `serialize` deviceIDCSR
+  );
+
+  (**) B.modifies_trans (B.loc_buffer deviceIDCRI_buf) h0 hs2 (B.loc_buffer deviceIDCSR_buf) hs3;
+  (**) let hsf = HST.get () in
+  HST.pop_frame ();
+  (**) let hf = HST.get () in
+  (**) B.popped_modifies hsf hf;
+  (**) B.modifies_buffer_elim deviceIDCSR_buf (B.loc_region_only false (HS.get_tip hsf)) hsf hf;
+  (**) B.modifies_fresh_frame_popped h0 hs0 (
+    B.loc_buffer deviceIDCSR_buf
+  ) hsf hf;
+()
+
+*)
+}
+```
